Implement zeroize_uds (works). progress on cdi_functional_correctness -- ran into issues changing array/seq -> larray/lseq throughout

pulse/share/steel/examples/pulse/dice/DICEEngineCore.fst
@@ -1,5 +1,6 @@
 module DICEEngineCore
 module A = Steel.ST.Array
+module R = Steel.ST.Reference
 module T = FStar.Tactics
 module PM = Pulse.Main
 open Steel.ST.Util 
@@ -19,10 +20,10 @@ assume
 val digest_len (_:alg_t) : US.t
 
 assume
-val spec_hash (a:alg_t) (s:Seq.seq U8.t) : Seq.lseq U8.t (US.v (digest_len a))
+val spec_hash (a:alg_t) (s:Seq.seq U8.t) : Ghost.erased (Seq.lseq U8.t (US.v (digest_len a)))
 
 assume
-val spec_hmac (a:alg_t) (k:Seq.seq U8.t) (m:Seq.seq U8.t) : Seq.lseq U8.t (US.v (digest_len a))
+val spec_hmac (a:alg_t) (k:Seq.seq U8.t) (m:Seq.seq U8.t) : Ghost.erased (Seq.lseq U8.t (US.v (digest_len a)))
 
 assume
 val is_hashable_len (_:US.t) : prop
@@ -40,8 +41,8 @@ val hacl_hash (alg:alg_t)
               (src_len: hashable_len { US.v src_len == A.length src })
               (dst:A.larray U8.t (US.v (digest_len alg)))
               (#psrc:perm)
-              (#src_seq:Ghost.erased (Seq.seq U8.t))
-              (#dst_seq:Ghost.erased (Seq.seq U8.t))
+              (#src_seq:Ghost.erased (Seq.lseq U8.t (US.v src_len)))
+              (#dst_seq:Ghost.erased (Seq.lseq U8.t (US.v (digest_len alg))))
   : stt unit
     (A.pts_to dst full_perm dst_seq `star`
      A.pts_to src psrc src_seq)
@@ -52,14 +53,14 @@ val hacl_hash (alg:alg_t)
 assume
 val hacl_hmac (alg:alg_t)
               (dst:A.larray U8.t (US.v (digest_len alg)))
-              (key:A.array U8.t)
-              (key_len: key_len { US.v key_len == A.length key })
-              (msg:A.array U8.t)
-              (msg_len: hashable_len { US.v msg_len == A.length msg })
+              (key_len: key_len)
+              (key:A.larray U8.t (US.v key_len))
+              (msg_len: hashable_len)
+              (msg:A.larray U8.t (US.v msg_len))
               (#pkey #pmsg:perm)
-              (#dst_seq:Ghost.erased (Seq.seq U8.t))
-              (#key_seq:Ghost.erased (Seq.seq U8.t))
-              (#msg_seq:Ghost.erased (Seq.seq U8.t))
+              (#dst_seq:Ghost.erased (Seq.lseq U8.t (US.v (digest_len alg))))
+              (#key_seq:Ghost.erased (Seq.lseq U8.t (US.v key_len)))
+              (#msg_seq:Ghost.erased (Seq.lseq U8.t (US.v msg_len)))
   : stt unit
     (A.pts_to dst full_perm dst_seq `star`
      A.pts_to key pkey key_seq `star`
@@ -85,6 +86,10 @@ assume
 val dice_digest_len_is_hashable 
   : is_hashable_len dice_digest_len
 
+assume
+val uds_len_dice_digest_len_equiv
+  : uds_len == dice_digest_len
+  
 type dice_return_code = | DICE_SUCCESS | DICE_ERROR
 
 let cdi_t = A.larray U8.t (US.v (digest_len dice_hash_alg))
@@ -110,18 +115,22 @@ let l0_perm (l0:l0_image_t) (vl0: l0_repr) : vprop =
     A.pts_to l0.l0_binary full_perm vl0.l0_binary
 
 assume
-val stack_is_erased : vprop
+// val uds_bytes : v:(Ghost.erased (Seq.seq U8.t)){ Seq.length v = US.v uds_len }
+val uds_bytes : Ghost.erased (Seq.lseq U8.t (US.v uds_len))
+
+(* currently not using *)
+// assume
+// val stack_is_erased : vprop
 
 assume
 val l0_is_authentic (vl0:l0_repr) : prop
 
-assume
-val cdi_functional_correctness (cdi:Seq.seq U8.t) (vl0:l0_repr) : prop
-// Roughly, we want to specify this predicate as
-// cdi == spec_hmac (spec_hash dice_hash_alg uds_bytes) (spec_hash ... l0_binary)
-
-assume
-val uds_bytes : Ghost.erased (Seq.seq U8.t)
+val cdi_functional_correctness 
+  (cdi:cdi_t) 
+  (l0:l0_image_t) 
+  (#c0:(c0:Ghost.erased (Seq.lseq U8.t (US.v uds_len)){uds_len == dice_digest_len}))
+  (#vl0:Ghost.erased l0_repr)
+  : c0 == spec_hmac dice_hash_alg (spec_hash dice_hash_alg uds_bytes) (spec_hash dice_hash_alg vl0.l0_binary)
 
 ```pulse
 fn authenticate_l0_image (l0:l0_image_t) (#vl0:Ghost.erased l0_repr)
@@ -132,7 +141,7 @@ fn authenticate_l0_image (l0:l0_image_t) (#vl0:Ghost.erased l0_repr)
         pure (b ==> l0_is_authentic vl0)
     )
 {
-    false //dummy; to be filled in with call to ED25519 etc
+  admit()
 }
 ```
 
@@ -149,24 +158,57 @@ fn disable_uds (_:unit)
 }
 ```
 
+let seq_constant_until (#t:Type) (s:Seq.seq t) (v:t) (n:nat) =
+    forall (i:nat). i < n /\ i < Seq.length s ==> Seq.index s i == v
 
-// assume
-// val compute_cdi (c:cdi_t) (l0:l0_image_t) (#vl0:Ghost.erased l0_repr)
-//   : stt unit  
-//      (exists_ (fun (c0:Seq.seq U8.t) ->
-//     uds_is_enabled `star`
-//     A.pts_to c full_perm c0 `star`
-//     l0_perm l0 vl0 (* should CDI only be computed on authentic l0 images? *)
-//     ))
-//     (fun _ ->   
-//           exists_ (fun (c1:Seq.seq U8.t) ->
-//             A.pts_to c full_perm c1 `star`
-//             l0_perm l0 vl0 `star`
-//             pure (cdi_functional_correctness c1 vl0)
-//           ))
+```pulse
+fn fill_array (#t:Type0) (a:A.array t) (l:(l:US.t { US.v l == A.length a })) (v:t)
+              (#s:(s:Ghost.erased (Seq.seq t) { Seq.length s == A.length a }))
+   requires (A.pts_to a full_perm s)
+   ensures 
+      exists (s:Seq.seq t). (
+         A.pts_to a full_perm s `star`
+         pure (seq_constant_until s v (US.v l))
+      )
+{
+   let mut i = 0sz;
+   while (let vi = !i; US.(vi <^ l))
+   invariant b. exists (s:Seq.seq t) (vi:US.t). ( 
+      A.pts_to a full_perm s `star`
+      R.pts_to i full_perm vi `star`
+      pure ((b == US.(vi <^ l)) /\
+            US.v vi <= US.v l /\
+            Seq.length s == A.length a /\
+            seq_constant_until s v (US.v vi))
+   )
+   {
+      let vi = !i; 
+      (a.(vi) <- v);
+      i := US.(vi +^ 1sz);
+      ()
+   };
+   ()
+}
+```
 
-
-
+```pulse
+fn zeroize_uds (uds:A.array U8.t) 
+               (l:(l:US.t{ US.v l = A.length uds })) 
+               (#uds0:(uds0:Ghost.erased (Seq.seq U8.t) { Seq.length uds0 = A.length uds }))
+  requires (
+    uds_is_enabled `star`
+    A.pts_to uds full_perm uds0
+  )
+  ensures (
+    uds_is_enabled `star`
+    (exists_ (fun (uds':Seq.seq U8.t) ->   
+      A.pts_to uds full_perm uds' `star`
+      pure (seq_constant_until uds' 0uy (US.v l))))
+  )
+{
+  fill_array uds l 0uy;
+}
+```
 
 assume
 val read_uds (uds:A.larray U8.t (US.v uds_len))
@@ -184,18 +226,23 @@ val free_array_u8
     (fun _ -> emp)
 
 ```pulse
-fn compute_cdi (c:cdi_t) (l0:l0_image_t) 
+fn compute_cdi (cdi:cdi_t) (l0:l0_image_t) 
                (#vl0:Ghost.erased l0_repr)
-               (#c0:Ghost.erased (Seq.seq U8.t))
+               (#c0:Ghost.erased (Seq.lseq U8.t (US.v uds_len)))
+               (#c1:Ghost.erased (Seq.lseq U8.t (US.v uds_len)))
  requires (
     uds_is_enabled `star`
-    A.pts_to c full_perm c0 `star`
+    A.pts_to cdi full_perm c0 `star`
     l0_perm l0 vl0 (* should CDI only be computed on authentic l0 images? *)
  )
- ensures exists (c1:Seq.seq U8.t). (
-    A.pts_to c full_perm c1 `star`
-    l0_perm l0 vl0 `star`
-    pure (cdi_functional_correctness c1 vl0)
+ ensures (
+  l0_perm l0 vl0 `star`
+  A.pts_to cdi full_perm c1 //`star`
+  (* cdi_functional_correctness cdi l0 #c1 #vl0 *)
+
+  // (exists_ (fun (c1:Seq.lseq U8.t (US.v uds_len)) -> (
+  //   A.pts_to cdi full_perm c1 `star`
+  //   cdi_functional_correctness cdi l0 #c1 #vl0)))
  )
 {
     let uds = new_array 0uy uds_len;
@@ -214,34 +261,39 @@ fn compute_cdi (c:cdi_t) (l0:l0_image_t)
 
     dice_digest_len_is_hashable;
 
-    hacl_hmac dice_hash_alg c 
-      uds_digest dice_digest_len
-      l0_digest dice_digest_len;
+    uds_len_dice_digest_len_equiv;
 
-    // zeroize uds_len uds;
+    hacl_hmac dice_hash_alg cdi
+      dice_digest_len uds_digest
+      dice_digest_len l0_digest;
+
+    // cdi_functional_correctness cdi l0 #c1 #vl0;
+
+    zeroize_uds uds uds_len;
 
     free_array l0_digest;
     free_array uds_digest;
     free_array uds;
     disable_uds();
-    admit()
+    // admit()
 }
 ```
 
 ```pulse
 fn dice_main (c:cdi_t) (l0:l0_image_t)
              (#vl0:Ghost.erased l0_repr)
-             (#c0:Ghost.erased (Seq.seq U8.t))
+             (#c0:Ghost.erased Seq.lseq U8.t (US.v uds_len))
   requires (
     uds_is_enabled `star`
     A.pts_to c full_perm c0 `star`
     l0_perm l0 vl0
   )
   returns r: dice_return_code
-  ensures exists (c1:Seq.seq U8.t). (
+  ensures exists (c1:Seq.lseq U8.t (US.v uds_len)). (
       A.pts_to c full_perm c1 `star`
       l0_perm l0 vl0 `star`
-      pure (r == DICE_SUCCESS ==> l0_is_authentic vl0 /\ cdi_functional_correctness c1 vl0)
+      cdi_functional_correctness c l0 `star`
+      pure (r == DICE_SUCCESS ==> l0_is_authentic vl0)
   )
 {
   let b = authenticate_l0_image l0;
@@ -258,7 +310,7 @@ fn dice_main (c:cdi_t) (l0:l0_image_t)
 }
 ```
 
-
+(*
 ```pulse
 fn compute_cdi_v2 (c:cdi_t) (l0:l0_image_t) (#vl0:Ghost.erased l0_repr)
  requires exists (c0: Seq.seq U8.t). (
@@ -309,3 +361,4 @@ fn dice_main_v2 (c:cdi_t) (l0:l0_image_t) (#vl0:Ghost.erased l0_repr)
   }
 }
 ```
+*)
